src/program_proof/mvcc/mvcc_inv.v
@@ -1,0 +1,116 @@
+From Perennial.program_proof Require Export grove_prelude.
+From Perennial.program_proof.mvcc Require Import mvcc_ghost proph_proof.
+
+(* Invariant namespaces. *)
+Definition mvccN := nroot.
+Definition mvccNTuple := nroot .@ "tuple".
+Definition mvccNGC := nroot .@ "gc".
+Definition mvccNSST := nroot .@ "sst".
+
+Section def.
+Context `{!heapGS Σ, !mvcc_ghostG Σ}.
+
+(* GC invariants. *)
+Definition mvcc_inv_gc_def γ : iProp Σ :=
+  [∗ list] sid ∈ sids_all,
+    ∃ (tids : gmap u64 unit) (tidmin : u64),
+      site_active_tids_half_auth γ sid tids ∗
+      site_min_tid_half_auth γ sid (int.nat tidmin) ∗
+      ∀ tid, ⌜tid ∈ (dom tids) -> (int.nat tidmin) ≤ (int.nat tid)⌝.
+
+Definition mvcc_inv_gc γ : iProp Σ :=
+  inv mvccNGC (mvcc_inv_gc_def γ).
+
+(* SST invariants. *)
+(* TODO *)
+Definition ptuple_past_rel (key : u64) (phys : list dbval) (past : list action) :=
+  True.
+
+Definition per_key_inv_def
+           (γ : mvcc_names) (key : u64) (tmods : gset (u64 * dbmap))
+           (m : dbmap) (past : list action)
+  : iProp Σ :=
+  ∃ (phys logi : list dbval),
+    "Hptuple" ∷ ptuple_auth γ (1 / 2) key phys ∗
+    "Hltuple" ∷ ltuple_auth γ key logi ∗
+    "%Htmrel" ∷ ⌜tuple_mods_rel phys logi (per_tuple_mods tmods key)⌝ ∗
+    "%Hpprel" ∷ ⌜ptuple_past_rel key phys past⌝ ∗
+    "%Hlmrel" ∷ ⌜last logi = m !! key⌝.
+
+Definition cmt_inv_def
+           (γ : mvcc_names) (tmods : gset (u64 * dbmap)) (future : list action)
+  : iProp Σ :=
+  "HcmtAuth" ∷ commit_tmods_auth γ tmods ∗
+  "%Hcmt"    ∷ ⌜set_Forall (uncurry (first_commit_compatible future)) tmods⌝.
+
+Definition nca_inv_def (γ : mvcc_names) (future : list action) : iProp Σ :=
+  ∃ (tids_nca : gset u64),
+    "HncaAuth" ∷ nca_tids_auth γ tids_nca ∗
+    "%Hnca"    ∷ ⌜set_Forall (no_commit_abort future) tids_nca⌝.
+
+Definition fa_inv_def (γ : mvcc_names) (future : list action) : iProp Σ :=
+  ∃ (tids_fa : gset u64),
+    "HfaAuth" ∷ fa_tids_auth γ tids_fa ∗
+    "%Hfa"    ∷ ⌜set_Forall (first_abort future) tids_fa⌝.
+
+Definition fci_inv_def (γ : mvcc_names) (past future : list action) : iProp Σ :=
+  ∃ (tmods_fci : gset (u64 * dbmap)),
+    "HfciAuth" ∷ fci_tmods_auth γ tmods_fci ∗
+    "%Hfci"    ∷ ⌜set_Forall (uncurry (first_commit_incompatible (past ++ future))) tmods_fci⌝.
+
+Definition fcc_inv_def (γ : mvcc_names) (future : list action) : iProp Σ :=
+  ∃ (tmods_fcc : gset (u64 * dbmap)),
+    "HfccAuth" ∷ fcc_tmods_auth γ tmods_fcc ∗
+    "%Hfcc"    ∷ ⌜set_Forall (uncurry (first_commit_compatible future)) tmods_fcc⌝.
+
+Definition mvcc_inv_sst_def γ p : iProp Σ :=
+  ∃ (tmods : gset (u64 * dbmap)) (m : dbmap) (past future : list action),
+    (* Prophcy. *)
+    "Hproph" ∷ mvcc_proph γ p future ∗
+    (* Global database map, i.e., auth element of the global ptsto. *)
+    "Hm" ∷ dbmap_auth γ m ∗
+    (* Per-key invariants. *)
+    "Hkeys" ∷ ([∗ set] key ∈ keys_all, per_key_inv_def γ key tmods m past) ∗
+    (* Ok txns. *)
+    "Hcmt"  ∷ cmt_inv_def γ tmods future ∗
+    (* Doomed txns. *)
+    "Hnca"  ∷ nca_inv_def γ future ∗
+    "Hfa"   ∷ fa_inv_def  γ future ∗
+    "Hfci"  ∷ fci_inv_def γ past future ∗
+    "Hfcc"  ∷ fcc_inv_def γ future.
+
+Instance mvcc_inv_sst_timeless γ p :
+  Timeless (mvcc_inv_sst_def γ p).
+Proof. unfold mvcc_inv_sst_def. apply _. Defined.
+
+Definition mvcc_inv_sst γ p : iProp Σ :=
+  inv mvccNSST (mvcc_inv_sst_def γ p).
+
+End def.
+
+Section theorem.
+Context `{!heapGS Σ, !mvcc_ghostG Σ}.
+
+Theorem active_ge_min γ (tid tidlb : u64) (sid : u64) :
+  mvcc_inv_gc_def γ -∗
+  active_tid γ tid sid -∗
+  min_tid_lb γ (int.nat tidlb) -∗
+  ⌜int.Z tidlb ≤ int.Z tid⌝.
+Proof using heapGS0 mvcc_ghostG0 Σ.
+  (* Q: How to remove [using]? *)
+  iIntros "Hinv Hactive Hlb".
+  iDestruct "Hactive" as "[[Htid %Hlookup] _]".
+  apply sids_all_lookup in Hlookup.
+  apply elem_of_list_lookup_2 in Hlookup.
+  iDestruct (big_sepL_elem_of with "Hlb") as "Htidlb"; first done.
+  iDestruct (big_sepL_elem_of with "Hinv") as (tids tidmin) "(Htids & Htidmin & %Hle)"; first done.
+  (* Obtaining [tidmin ≤ tid]. *)
+  iDestruct (site_active_tids_elem_of with "Htids Htid") as "%Helem".
+  apply Hle in Helem.
+  (* Obtaining [tidlb ≤ tidmin]. *)
+  iDestruct (site_min_tid_valid with "Htidmin Htidlb") as "%Hle'".
+  iPureIntro.
+  apply Z.le_trans with (int.Z tidmin); word.
+Qed.
+
+End theorem.
