src/program_proof/mvcc/proph_proof.v
@@ -10,17 +10,27 @@ Context `{!heapGS Σ}.
 Definition mvcc_proph (γ : mvcc_names) (p : proph_id) (acs : list action) : iProp Σ.
 Admitted.
 
+Global Instance mvcc_proph_timeless γ p acs :
+  Timeless (mvcc_proph γ p acs).
+Admitted.
+
+Lemma wp_NewProphActions γ :
+  {{{ True }}}
+    NewProph #()
+  {{{ (p : proph_id) acs, RET #p; mvcc_proph γ p acs }}}.
+Admitted.
+
 Lemma wp_ResolveRead γ p (tid key : u64) :
   ⊢ <<< ∀∀ acs, mvcc_proph γ p acs >>>
       ResolveRead #p #tid #key @ ∅
-    <<< ∃ acs', ⌜acs = EvRead tid key :: acs⌝ ∗ mvcc_proph γ p acs' >>>
+    <<< ∃ acs', ⌜acs = EvRead tid key :: acs'⌝ ∗ mvcc_proph γ p acs' >>>
     {{{ RET #(); True }}}.
 Admitted.
 
 Lemma wp_ResolveAbort γ p (tid : u64) :
   ⊢ <<< ∀∀ acs, mvcc_proph γ p acs >>>
       ResolveAbort #p #tid @ ∅
-    <<< ∃ acs', ⌜acs = EvAbort tid :: acs⌝ ∗ mvcc_proph γ p acs' >>>
+    <<< ∃ acs', ⌜acs = EvAbort tid :: acs'⌝ ∗ mvcc_proph γ p acs' >>>
     {{{ RET #(); True }}}.
 Admitted.
 
