src/program_proof/mvcc/grepv.sh
@@ -1,0 +1,3 @@
+#!/bin/bash
+
+grep ${1} -r ${2} --include \*.v
